Docstrings for all functions and definitions in `SplayMap.lean` and module docstrings in `SortedMap.lean` and `SortedTree.lean` completed. Further progress on `SplayMap.lean`. API in other files still needs to be updated.

SplayTree4Lean/SortedTree.lean
@@ -1,58 +1,68 @@
-import SplayTree4Lean.SplayMap
+import SortedTree4Lean.SplayMap
 
 universe u
 variable {α : Type u} [LinearOrder α]
 
-def SplayTree (α : Type u) := SplayMap α Unit
+/-! A formal implementation of Splay trees. These are implemented using dynamic self-balancing search trees, modified mainly by a `splay` operation, attributed to Sleator and Tardos (https://www.cs.cmu.edu/~sleator/papers/self-adjusting.pdf).
 
-instance [DecidableEq α] : DecidableEq (SplayTree α) :=
+API offered by this module:
+- `SortedTree α β` is a splay tree with `key`s of type `α` with a `LinearOrder` instance, and `value`s of type `β`.
+- `SortedMap.nil` is the empty tree.
+- `search` is a function that takes a `SortedMap α β` and a key `x : α`, and returns the tree with `x` splayed to the root. Even if `x` is not in the tree, the output tree may still be modified.
+- `insert` is a function that takes a `SortedMap α β`, a key `xk : α`, a value `xv : β`, and returns the tree with `(xk, xv)` inserted. If `xk` is already in the tree, the value is updated.
+- `delete` is a function that takes a `SortedMap α β` and a key `x : α`, and returns the tree with `x` deleted. If `x` is not in the input tree, the output tree may still be modified.
+ -/
+
+def SortedTree (α : Type u) := SplayMap α Unit
+
+instance [DecidableEq α] : DecidableEq (SortedTree α) :=
   inferInstanceAs (DecidableEq (SplayMap α Unit))
 
-namespace SplayTree
+namespace SortedTree
 
-def nil : SplayTree α :=
+def nil : SortedTree α :=
   SplayMap.nil
-def node (xk : α) : SplayTree α → SplayTree α → SplayTree α :=
+def node (xk : α) : SortedTree α → SortedTree α → SortedTree α :=
   SplayMap.node xk .unit
 
-def toStr [ToString α] (header : String) : SplayTree α → String
+def toStr [ToString α] (header : String) : SortedTree α → String
   | SplayMap.nil => header ++ "nil\n"
   | SplayMap.node yk _ yL yR => header ++ toString yk ++ "\n" ++ toStr header' yL ++ toStr header' yR
       where header' := header ++ "    "
 
-instance [ToString α] : ToString (SplayTree α) :=
+instance [ToString α] : ToString (SortedTree α) :=
   ⟨toStr ""⟩
 
-instance instSplayTreeMem : Membership α (SplayTree α) :=
+instance instSortedTreeMem : Membership α (SortedTree α) :=
   inferInstanceAs (Membership α (SplayMap α Unit))
 
 #synth DecidableEq (SplayMap Nat Unit)
-#synth DecidableEq (SplayTree Nat)
+#synth DecidableEq (SortedTree Nat)
 
-def insert (t : SplayTree α) (xk : α) : SplayTree α :=
+def insert (t : SortedTree α) (xk : α) : SortedTree α :=
   SplayMap.insert t xk Unit.unit
 
-def delete : SplayTree α → α → SplayTree α :=
+def delete : SortedTree α → α → SortedTree α :=
   SplayMap.delete
 
-def fromList : List α → SplayTree α :=
+def fromList : List α → SortedTree α :=
   SplayMap.fromList ∘ List.map (fun x => (x, Unit.unit))
 
-def toList : SplayTree α → List α :=
+def toList : SortedTree α → List α :=
   List.map (fun (x, _) => x) ∘ SplayMap.toList
 
-end SplayTree
+end SortedTree
 
 section demo
-open SplayTree
+open SortedTree
 
-def exampleTree1 : SplayTree Nat :=
+def exampleTree1 : SortedTree Nat :=
   -- insert 10 (insert 20 (insert 30 (insert 25 (insert 5 (insert (15 : ℕ) nil)))))
   (((((nil.insert 15).insert 5).insert 25).insert 30).insert 20).insert 10
 
 def L : List Nat := [5, 3, 8, 1, 4, 7, 9]
 
-def exampleTree2 : SplayTree Nat :=
+def exampleTree2 : SortedTree Nat :=
   fromList L
 
 #eval exampleTree1
@@ -64,7 +74,7 @@ def exampleTree2 : SplayTree Nat :=
 /-! Time for some unit testing. -/
 
 -- The subtree of the infinite complete binary tree with r at the root
-def ctf (r : Nat) : SplayTree Nat :=
+def ctf (r : Nat) : SortedTree Nat :=
   let h := Nat.maxPowDiv 2 r
   if h = 0 then
     node r nil nil
@@ -73,14 +83,14 @@ def ctf (r : Nat) : SplayTree Nat :=
 termination_by Nat.maxPowDiv 2 r
 decreasing_by sorry; sorry -- why do I need two of them?
 
-def tree4 : SplayTree Nat := ctf 4
+def tree4 : SortedTree Nat := ctf 4
 #eval! tree4
 #eval! find tree4 4 -- root
 #eval! find tree4 2 -- zig
 #eval! find tree4 1 -- ziz-zig
 #eval! find tree4 3 -- zig-zag
 
-def tree16 : SplayTree Nat := ctf (16 : Nat)
+def tree16 : SortedTree Nat := ctf (16 : Nat)
 #eval! tree16
 #eval! tree16.find 8
 #eval! tree16.find 4
